tuned (using anonymous context to capture "key" function)

thys/Efficient-Mergesort/Efficient_Mergesort.thy
@@ -15,91 +15,66 @@ text \<open>
   data suggests that generated code for this implementation is much more
   efficient than for the implementation provided by \<^theory>\<open>HOL-Library.Multiset\<close>.
 \<close>
-context linorder
-begin
-
-
 subsection \<open>Definition of Natural Mergesort\<close>
+
+context
+  fixes key :: "'a \<Rightarrow> 'k::linorder"
+begin
 
 text \<open>
   Split a list into chunks of ascending and descending parts, where
   descending parts are reversed on the fly.
   Thus, the result is a list of sorted lists.
 \<close>
-fun sequences :: "('b \<Rightarrow> 'a) \<Rightarrow> 'b list \<Rightarrow> 'b list list"
-  and asc :: "('b \<Rightarrow> 'a) \<Rightarrow> 'b \<Rightarrow> ('b list \<Rightarrow> 'b list) \<Rightarrow> 'b list \<Rightarrow> 'b list list"
-  and desc :: "('b \<Rightarrow> 'a) \<Rightarrow> 'b \<Rightarrow> 'b list \<Rightarrow> 'b list \<Rightarrow> 'b list list"
+fun sequences :: "'a list \<Rightarrow> 'a list list"
+  and asc :: "'a \<Rightarrow> ('a list \<Rightarrow> 'a list) \<Rightarrow> 'a list \<Rightarrow> 'a list list"
+  and desc :: "'a \<Rightarrow> 'a list \<Rightarrow> 'a list \<Rightarrow> 'a list list"
   where
-    "sequences key (a # b # xs) =
-      (if key a > key b then desc key b [a] xs else asc key b ((#) a) xs)"
-  | "sequences key [x] = [[x]]"
-  | "sequences key [] = []"
-  | "asc key a f (b # bs) =
-      (if \<not> key a > key b then asc key b (f \<circ> (#) a) bs
-      else f [a] # sequences key (b # bs))"
-  | "asc key a f [] = [f [a]]"
-  | "desc key a as (b # bs) =
-      (if key a > key b then desc key b (a # as) bs
-      else (a # as) # sequences key (b # bs))"
-  | "desc key a as [] = [a # as]"
+    "sequences (a # b # xs) =
+      (if key a > key b then desc b [a] xs else asc b ((#) a) xs)"
+  | "sequences [x] = [[x]]"
+  | "sequences [] = []"
+  | "asc a f (b # bs) =
+      (if \<not> key a > key b then asc b (f \<circ> (#) a) bs
+      else f [a] # sequences (b # bs))"
+  | "asc a f [] = [f [a]]"
+  | "desc a as (b # bs) =
+      (if key a > key b then desc b (a # as) bs
+      else (a # as) # sequences (b # bs))"
+  | "desc a as [] = [a # as]"
 
-fun merge :: "('b \<Rightarrow> 'a) \<Rightarrow> 'b list \<Rightarrow> 'b list \<Rightarrow> 'b list"
+fun merge :: "'a list \<Rightarrow> 'a list \<Rightarrow> 'a list"
   where
-    "merge key (a#as) (b#bs) =
-      (if key a > key b then b # merge key (a#as) bs
-      else a # merge key as (b#bs))"
-  | "merge key [] bs = bs"
-  | "merge key as [] = as"
+    "merge (a # as) (b # bs) =
+      (if key a > key b then b # merge (a # as) bs else a # merge as (b # bs))"
+  | "merge [] bs = bs"
+  | "merge as [] = as"
 
-fun merge_pairs :: "('b \<Rightarrow> 'a) \<Rightarrow> 'b list list \<Rightarrow> 'b list list"
+fun merge_pairs :: "'a list list \<Rightarrow> 'a list list"
   where
-    "merge_pairs key (a#b#xs) = merge key a b # merge_pairs key xs"
-  | "merge_pairs key xs = xs"
+    "merge_pairs (a # b # xs) = merge a b # merge_pairs xs"
+  | "merge_pairs xs = xs"
 
 lemma length_merge [simp]:
-  "length (merge key xs ys) = length xs + length ys"
+  "length (merge xs ys) = length xs + length ys"
   by (induct xs ys rule: merge.induct) simp_all
 
-lemma length_merge_pairs [termination_simp]:
-  "length (merge_pairs key xs) \<le> length xs"
-  by (induct key xs rule: merge_pairs.induct) simp_all
+lemma length_merge_pairs [simp]:
+  "length (merge_pairs xs) = (1 + length xs) div 2"
+  by (induct xs rule: merge_pairs.induct) simp_all
 
-fun merge_all :: "('b \<Rightarrow> 'a) \<Rightarrow> 'b list list \<Rightarrow> 'b list"
+fun merge_all :: "'a list list \<Rightarrow> 'a list"
   where
-    "merge_all key [] = []"
-  | "merge_all key [x] = x"
-  | "merge_all key xs = merge_all key (merge_pairs key xs)"
+    "merge_all [] = []"
+  | "merge_all [x] = x"
+  | "merge_all xs = merge_all (merge_pairs xs)"
 
-fun msort_key :: "('b \<Rightarrow> 'a) \<Rightarrow> 'b list \<Rightarrow> 'b list"
+fun msort_key :: "'a list \<Rightarrow> 'a list"
   where
-    "msort_key key xs = merge_all key (sequences key xs)"
+    "msort_key xs = merge_all (sequences xs)"
 
 
-subsection \<open>Functional Correctness\<close>
-
-lemma mset_merge [simp]:
-  "mset (merge key xs ys) = mset xs + mset ys"
-  by (induct xs ys rule: merge.induct) (simp_all add: ac_simps)
-
-lemma set_merge [simp]:
-  "set (merge key xs ys) = set xs \<union> set ys"
-  by (simp flip: set_mset_mset)
-
-lemma mset_concat_merge_pairs [simp]:
-  "mset (concat (merge_pairs key xs)) = mset (concat xs)"
-  by (induct key xs rule: merge_pairs.induct) (auto simp: ac_simps)
-
-lemma set_concat_merge_pairs [simp]:
-  "set (concat (merge_pairs key xs)) = set (concat xs)"
-  by (simp flip: set_mset_mset)
-
-lemma mset_merge_all [simp]:
-  "mset (merge_all key xs) = mset (concat xs)"
-  by (induct key xs rule: merge_all.induct) (simp_all add: ac_simps)
-
-lemma set_merge_all [simp]:
-  "set (merge_all key xs) = set (concat xs)"
-  by (simp flip: set_mset_mset)
+subsection \<open>Facts about Lengths\<close>
 
 definition "ascP f = (\<forall>xs ys. f (xs @ ys) = f xs @ ys)"
 
@@ -121,67 +96,100 @@ lemma ascP_f_Cons:
   shows "f (x # xs) = f [] @ x # xs"
   using assms [unfolded ascP_def, THEN spec, THEN spec, of "[]" "x # xs"] by simp
 
-lemma mset_sequences [simp]:
-  "mset (concat (sequences key xs)) = mset xs"
-  "ascP f \<Longrightarrow> mset (concat (asc key x f ys)) = {#x#} + mset (f []) + mset ys"
-  "mset (concat (desc key x xs ys)) = {#x#} + mset xs + mset ys"
-  by (induct key xs and key x f ys and key x xs ys rule: sequences_asc_desc.induct)
+lemma
+  shows length_sequences: "length (sequences xs) \<le> length xs"
+    and length_asc: "ascP f \<Longrightarrow> length (asc a f ys) \<le> 1 + length ys"
+    and length_desc: "length (desc a xs ys) \<le> 1 + length ys"
+  by (induct xs and a f ys and a xs ys rule: sequences_asc_desc.induct) auto
+
+lemma length_concat_merge_pairs [simp]:
+  "length (concat (merge_pairs xss)) = length (concat xss)"
+  by (induct xss rule: merge_pairs.induct) simp_all
+
+
+subsection \<open>Functional Correctness\<close>
+
+lemma mset_merge [simp]:
+  "mset (merge xs ys) = mset xs + mset ys"
+  by (induct xs ys rule: merge.induct) (simp_all add: ac_simps)
+
+lemma set_merge [simp]:
+  "set (merge xs ys) = set xs \<union> set ys"
+  by (simp flip: set_mset_mset)
+
+lemma mset_concat_merge_pairs [simp]:
+  "mset (concat (merge_pairs xs)) = mset (concat xs)"
+  by (induct xs rule: merge_pairs.induct) (auto simp: ac_simps)
+
+lemma set_concat_merge_pairs [simp]:
+  "set (concat (merge_pairs xs)) = set (concat xs)"
+  by (simp flip: set_mset_mset)
+
+lemma mset_merge_all [simp]:
+  "mset (merge_all xs) = mset (concat xs)"
+  by (induct xs rule: merge_all.induct) (simp_all add: ac_simps)
+
+lemma set_merge_all [simp]:
+  "set (merge_all xs) = set (concat xs)"
+  by (simp flip: set_mset_mset)
+
+lemma
+  shows mset_seqeuences [simp]: "mset (concat (sequences xs)) = mset xs"
+    and mset_asc: "ascP f \<Longrightarrow> mset (concat (asc x f ys)) = {#x#} + mset (f []) + mset ys"
+    and mset_desc: "mset (concat (desc x xs ys)) = {#x#} + mset xs + mset ys"
+  by (induct xs and x f ys and x xs ys rule: sequences_asc_desc.induct)
     (auto simp: ascP_f_singleton)
 
 lemma mset_msort_key:
-  "mset (msort_key key xs) = mset xs"
+  "mset (msort_key xs) = mset xs"
   by (auto)
 
 lemma sorted_merge [simp]:
   assumes "sorted (map key xs)" and "sorted (map key ys)"
-  shows "sorted (map key (merge key xs ys))"
-  using assms by (induct key xs ys rule: merge.induct) (auto)
+  shows "sorted (map key (merge xs ys))"
+  using assms by (induct xs ys rule: merge.induct) (auto)
 
 lemma sorted_merge_pairs [simp]:
   assumes "\<forall>x\<in>set xs. sorted (map key x)"
-  shows "\<forall>x\<in>set (merge_pairs key xs). sorted (map key x)"
-  using assms by (induct key xs rule: merge_pairs.induct) simp_all
+  shows "\<forall>x\<in>set (merge_pairs xs). sorted (map key x)"
+  using assms by (induct xs rule: merge_pairs.induct) simp_all
 
 lemma sorted_merge_all:
   assumes "\<forall>x\<in>set xs. sorted (map key x)"
-  shows "sorted (map key (merge_all key xs))"
-  using assms by (induct key xs rule: merge_all.induct) simp_all
+  shows "sorted (map key (merge_all xs))"
+  using assms by (induct xs rule: merge_all.induct) simp_all
 
 lemma
-  shows sorted_sequences: "\<forall>x \<in> set (sequences key xs). sorted (map key x)"
-    and sorted_asc: "ascP f \<Longrightarrow> sorted (map key (f [])) \<Longrightarrow> \<forall>x\<in>set (f []). key x \<le> key a \<Longrightarrow> \<forall>x\<in>set (asc key a f ys). sorted (map key x)"
-    and sorted_desc: "sorted (map key xs) \<Longrightarrow> \<forall>x\<in>set xs. key a \<le> key x \<Longrightarrow> \<forall>x\<in>set (desc key a xs ys). sorted (map key x)"
-  by (induct key xs and key a f ys and key a xs ys rule: sequences_asc_desc.induct)
+  shows sorted_sequences: "\<forall>x \<in> set (sequences xs). sorted (map key x)"
+    and sorted_asc: "ascP f \<Longrightarrow> sorted (map key (f [])) \<Longrightarrow> \<forall>x\<in>set (f []). key x \<le> key a \<Longrightarrow> \<forall>x\<in>set (asc a f ys). sorted (map key x)"
+    and sorted_desc: "sorted (map key xs) \<Longrightarrow> \<forall>x\<in>set xs. key a \<le> key x \<Longrightarrow> \<forall>x\<in>set (desc a xs ys). sorted (map key x)"
+  by (induct xs and a f ys and a xs ys rule: sequences_asc_desc.induct)
     (auto simp: ascP_f_singleton sorted_append not_less dest: order_trans, fastforce)
 
 lemma sorted_msort_key:
-  "sorted (map key (msort_key key xs))"
+  "sorted (map key (msort_key xs))"
   by (unfold msort_key.simps) (intro sorted_merge_all sorted_sequences)
 
 
 subsection \<open>Stability\<close>
 
 lemma
-  shows filter_by_key_sequences [simp]:
-    "[y\<leftarrow>concat (sequences key xs). key y = k] = [y\<leftarrow>xs. key y = k]"
-    and filter_by_key_asc:
-    "ascP f \<Longrightarrow> [y\<leftarrow>concat (asc key a f ys). key y = k] = [y\<leftarrow>f [a] @ ys. key y = k]"
-    and filter_by_key_desc:
-    "sorted (map key xs) \<Longrightarrow> \<forall>x\<in>set xs. key a \<le> key x \<Longrightarrow> [y\<leftarrow>concat (desc key a xs ys). key y = k] = [y\<leftarrow>a # xs @ ys. key y = k]"
-proof (induct key xs and key a f ys and key a xs ys rule: sequences_asc_desc.induct)
-  case (4 key a f b bs)
+  shows filter_by_key_sequences [simp]: "[y\<leftarrow>concat (sequences xs). key y = k] = [y\<leftarrow>xs. key y = k]"
+    and filter_by_key_asc: "ascP f \<Longrightarrow> [y\<leftarrow>concat (asc a f ys). key y = k] = [y\<leftarrow>f [a] @ ys. key y = k]"
+    and filter_by_key_desc: "sorted (map key xs) \<Longrightarrow> \<forall>x\<in>set xs. key a \<le> key x \<Longrightarrow> [y\<leftarrow>concat (desc a xs ys). key y = k] = [y\<leftarrow>a # xs @ ys. key y = k]"
+proof (induct xs and a f ys and a xs ys rule: sequences_asc_desc.induct)
+  case (4 a f b bs)
   then show ?case
     by (auto simp: o_def ascP_f_Cons [where f = f] ascP_comp_Cons')
 next
-  case (6 key a as b bs)
+  case (6 a as b bs)
   then show ?case
   proof (cases "key b < key a")
     case True
-    with 6 have "[y\<leftarrow>concat (desc key b (a # as) bs). key y = k] =
-      [y\<leftarrow>b # (a # as) @ bs. key y = k]"
-      by  (auto) (insert dual_order.order_iff_strict dual_order.trans, blast+)
+    with 6 have "[y\<leftarrow>concat (desc b (a # as) bs). key y = k] = [y\<leftarrow>b # (a # as) @ bs. key y = k]"
+      by (auto simp: less_le order_trans)
     moreover
-    from 6 have "\<forall>x\<in>set (desc key a as (b # bs)). sorted (map key x)" by (intro sorted_desc)
+    from 6 have "\<forall>x\<in>set (desc a as (b # bs)). sorted (map key x)" by (intro sorted_desc)
     ultimately show ?thesis
       using True and 6 by (auto simp: Cons_eq_append_conv intro!: filter_False)
   qed auto
@@ -189,41 +197,40 @@ qed auto
  
 lemma filter_by_key_merge_is_append [simp]:
   assumes "sorted (map key xs)"
-  shows "[y\<leftarrow>merge key xs ys. key y = k] = [y\<leftarrow>xs. key y = k] @ [y\<leftarrow>ys. key y = k]"
+  shows "[y\<leftarrow>merge xs ys. key y = k] = [y\<leftarrow>xs. key y = k] @ [y\<leftarrow>ys. key y = k]"
   using assms
-  by (induct key xs ys rule: merge.induct)
-    (auto simp: Cons_eq_append_conv leD intro!: filter_False)
+  by (induct xs ys rule: merge.induct) (auto simp: Cons_eq_append_conv leD intro!: filter_False)
 
 lemma filter_by_key_merge_pairs [simp]:
   assumes "\<forall>xs\<in>set xss. sorted (map key xs)"
-  shows "[y\<leftarrow>concat (merge_pairs key xss). key y = k] = [y\<leftarrow>concat xss. key y = k]"
-  using assms by (induct key xss rule: merge_pairs.induct) simp_all
+  shows "[y\<leftarrow>concat (merge_pairs xss). key y = k] = [y\<leftarrow>concat xss. key y = k]"
+  using assms by (induct xss rule: merge_pairs.induct) simp_all
 
 lemma filter_by_key_merge_all [simp]:
   assumes "\<forall>xs\<in>set xss. sorted (map key xs)"
-  shows "[y\<leftarrow>merge_all key xss. key y = k] = [y\<leftarrow>concat xss. key y = k]"
-  using assms by (induct key xss rule: merge_all.induct) simp_all
+  shows "[y\<leftarrow>merge_all xss. key y = k] = [y\<leftarrow>concat xss. key y = k]"
+  using assms by (induct xss rule: merge_all.induct) simp_all
 
 lemma filter_by_key_merge_all_sequences [simp]:
-  "[x\<leftarrow>merge_all key (sequences key xs) . key x = k] = [x\<leftarrow>xs . key x = k]"
-  using sorted_sequences [of key xs] by simp
+  "[x\<leftarrow>merge_all (sequences xs) . key x = k] = [x\<leftarrow>xs . key x = k]"
+  using sorted_sequences [of xs] by simp
 
 lemma msort_key_stable:
-  "[x\<leftarrow>msort_key key xs. key x = k] = [x\<leftarrow>xs. key x = k]"
+  "[x\<leftarrow>msort_key xs. key x = k] = [x\<leftarrow>xs. key x = k]"
   by auto
 
 lemma sort_key_msort_key_conv:
-  "sort_key key = msort_key key"
-  using msort_key_stable [of key "key x" for key x, of key]
+  "sort_key key = msort_key"
+  using msort_key_stable [of "key x" for x]
   by (intro ext properties_for_sort_key mset_msort_key sorted_msort_key)
     (metis (mono_tags, lifting) filter_cong)
 
+end
+
 text \<open>
-  Replace existing code equations for \<^const>\<open>sort_key\<close> by \<^term>\<open>msort_key key\<close>.
+  Replace existing code equations for \<^const>\<open>sort_key\<close> by \<^const>\<open>msort_key\<close>.
 \<close>
 declare sort_key_by_quicksort_code [code del]
 declare sort_key_msort_key_conv [code]
-
-end
 
 end
